coq/denot/subst.v
@@ -1,0 +1,140 @@
+(* 
+
+The weakening and substitution properties for denot.
+   
+Lemma weaken_denot : forall t ρ2 ρ,
+   fv_tm t [<=] dom ρ2 ->
+   uniq (ρ ++ ρ2) ->
+   denot t ρ2 = denot t (ρ ++ ρ2). 
+
+Lemma subst_denot1 :
+  forall (t : tm) (x : atom) (u : tm) (ρ : Env (P Value)),
+    scoped t (x ~ denot u ρ ++ ρ) ->
+    scoped u ρ ->
+    denot t (x ~ denot u ρ ++ ρ) = denot (t [x ~> u]) ρ.
+
+ *)
+
+
+Require Import Coq.Logic.FunctionalExtensionality.
+Require Import Coq.Classes.RelationClasses.
+Require Coq.Relations.Relation_Definitions.
+Require Import Lia.
+
+Require Export lc.tactics.
+Require Import lc.scoped.
+
+Require Import structures.Structures.
+Require Import denot.definitions.
+Require Import denot.denot.
+
+Import SetNotations.
+Local Open Scope set_scope.
+Import MonadNotation.
+Open Scope monad_scope.
+
+Import EnvNotations.
+Import LCNotations.
+
+Import Wf_nat.
+
+Lemma weaken_access {x}{ρ1 ρ ρ2}:
+  singleton x [<=] union (dom ρ1) (dom ρ2) ->
+  uniq (ρ1 ++ ρ ++ ρ2) ->
+  (ρ1 ++ ρ2) ⋅ x = (ρ1 ++ ρ ++ ρ2) ⋅ x.
+Proof.
+  intros FV U.
+  destruct_uniq.
+  move: (access_app_P ρ1 x) => [A1|A2].
+  rewrite A1. rewrite A1. auto.
+  move: (A2 ρ2) => [A21 A22].
+  rewrite A22.
+  move: (A2 (ρ ++ ρ2)) => [A31 A32].
+  rewrite A32.
+  rewrite access_app_fresh; auto.
+  intro h.
+  solve_uniq.
+Qed.
+
+Lemma weaken_denot1 : forall t ρ ρ1 ρ2, 
+    fv_tm t [<=] dom (ρ1 ++ ρ2) ->
+    uniq (ρ1 ++ ρ ++ ρ2) ->
+    denot t (ρ1 ++ ρ2) = denot t (ρ1 ++ ρ ++ ρ2). 
+Proof.
+  intro t.
+  eapply tm_induction with (t := t).
+  1: move=>i. 
+  2: move=>x.
+  3: move=>t1 t2 IH1 IH2. 
+  4: move=> u IH.
+  8: move=> t1 t2 IH1 IH2.
+  all: intros ρ ρ1 ρ2 FV U.
+  all: simpl_env in FV; simpl in FV. 
+  all: autorewrite with denot.
+  all: try solve [reflexivity].
+  + (* var *) 
+    f_equal.
+    eapply weaken_access; eauto.
+  + (* app *)
+    f_equal.
+    eapply IH1; simpl_env; eauto.
+    fsetdec.
+    extensionality v1. f_equal.
+    eapply IH2; simpl_env; eauto.
+    fsetdec.
+  + pick fresh x.
+    repeat rewrite (denot_abs x).
+    simpl_env; fsetdec.
+    simpl_env; fsetdec.
+    f_equal. f_equal.
+    extensionality D.
+    rewrite <- app_assoc.
+    erewrite IH; simpl_env; eauto.
+    rewrite fv_tm_open_tm_wrt_tm_upper; simpl; eauto.
+    fsetdec.
+  + f_equal.
+    eapply IH1; simpl_env; eauto.
+    fsetdec.
+    extensionality v1. 
+    f_equal.
+    eapply IH2; simpl_env; eauto.
+    fsetdec.
+Qed.
+
+Lemma weaken_denot : forall t ρ2 ρ,
+   fv_tm t [<=] dom ρ2 ->
+   uniq (ρ ++ ρ2) ->
+   denot t ρ2 = denot t (ρ ++ ρ2). 
+Proof.
+  intros.
+  unfold denot.
+  eapply weaken_denot1 with (ρ1 := nil); simpl; auto.
+Qed.
+
+
+Lemma weaken_denot_val : forall t ρ2 ρ,
+   fv_tm t [<=] dom ρ2 ->
+   uniq (ρ ++ ρ2) ->
+   denot_val t ρ2 = denot_val t (ρ ++ ρ2). 
+Proof.
+  intros.
+  induction t.
+  all: autorewrite with denot.
+  all: try reflexivity.
+  + move: (@weaken_access x nil ρ ρ2) => WA. 
+    eapply WA; eauto. simpl in H. fsetdec.
+  + pick fresh x.
+    repeat rewrite (denot_val_abs x); simpl_env; try fsetdec.
+    f_equal.
+    extensionality D.
+    eapply weaken_denot1.
+    rewrite fv_tm_open_tm_wrt_tm_upper; simpl; eauto.
+    fsetdec.
+    solve_uniq.
+  + simpl in H.
+    f_equal. 
+    eapply IHt1; eauto. fsetdec.
+    eapply IHt2; eauto. fsetdec.
+Qed.
+
+
