coq/denot/valid_theory.v
@@ -92,7 +92,7 @@ Lemma valid_ADD : valid ADD.
 Proof. 
   unfold ADD, valid.
   exists ( (v_list (v_nat 0 :: v_nat 0 :: nil) :: nil) ↦ pure_Comp ((v_nat 0) :: nil)). 
-  exists 0. exists 0. split.  auto. auto.
+  exists 0. exists 0. exists 0. repeat split; auto. 
 Qed.
 
 Lemma valid_Λ : forall F, valid (Λ F).
